\documentclass{article}
\usepackage{amsfonts}
\usepackage{amsmath}
\usepackage{amssymb}
\usepackage{setspace}
\begin{document}
\begin{spacing}{2.0}
\noindent
\textbf{Exercise 3.2-7:}\\
$
\phi = \frac{1 + \sqrt{5}}{2}\\
\hat{\phi} = \frac{1 - \sqrt{5}}{2}\\
\therefore F_1 = \frac{\phi - \hat{\phi}}{\sqrt{5}} = 1\\
\therefore F_2 = \frac{\phi ^ 2 - \hat{\phi} ^ 2}{\sqrt{5}} = 2\\
\therefore Let's\ suppose\ F_n = \frac{\phi ^ n - \hat{\phi} ^ n}{\sqrt{5}}\\
\therefore F_{n - 1} = \frac{\phi ^ {n - 1} - \hat{\phi} ^ {n - 1}}{\sqrt{5}}\\
\begin{aligned}
\therefore F_{n + 1} &= F_{n - 1} + F_n\\
&= \frac{\phi ^ {n - 1} \cdot \frac{3 + \sqrt{5}}{2} - \hat{\phi} ^ {n - 1} \cdot \frac{3 - \sqrt{5}}{2}}{\sqrt{5}}\\
&= \frac{\phi ^ {n + 1} - \hat{\phi} ^ {n + 1}}{\sqrt{5}}
\end{aligned}\\
\therefore F_{n + 1} = \frac{\phi ^ {n + 1} - \hat{\phi} ^ {n + 1}}{\sqrt{5}}\\
\therefore The\ induction\ holds\ for\ n = N + 1\\
\therefore F_i = \frac{\phi ^ i - \hat{\phi} ^ i}{\sqrt{5}}\\
$
\end{spacing}
\end{document}
